Impl/EvictModel.i.dfy
@@ -96,7 +96,7 @@ module EvictModel {
   ensures ValidDiskOp(diskOp(io'))
   ensures
     || BBC.Next(Ik(k).bc, IBlockCache(s), IBlockCache(s'), IDiskOp(diskOp(io')).bdop, StatesInternalOp)
-    || BBC.Next(Ik(k).bc, IBlockCache(s), IBlockCache(s'), IDiskOp(diskOp(io')).bdop, AdvanceOp(UI.NoOp, false))
+    || BBC.Next(Ik(k).bc, IBlockCache(s), IBlockCache(s'), IDiskOp(diskOp(io')).bdop, AdvanceOp(UI.NoOp, true))
   {
     var ref := FindDeallocable(s);
     FindDeallocableCorrect(s);
@@ -150,7 +150,7 @@ module EvictModel {
   ensures ValidDiskOp(diskOp(io'))
   ensures
     || BBC.Next(Ik(k).bc, IBlockCache(s), IBlockCache(s'), IDiskOp(diskOp(io')).bdop, StatesInternalOp)
-    || BBC.Next(Ik(k).bc, IBlockCache(s), IBlockCache(s'), IDiskOp(diskOp(io')).bdop, AdvanceOp(UI.NoOp, false))
+    || BBC.Next(Ik(k).bc, IBlockCache(s), IBlockCache(s'), IDiskOp(diskOp(io')).bdop, AdvanceOp(UI.NoOp, true))
   {
     reveal_PageInNodeReqOrMakeRoom();
 
