Impl/GrowModel.i.dfy
@@ -4,6 +4,7 @@ module GrowModel {
   import opened StateModel
   import opened IOModel
   import opened BookkeepingModel
+  import opened ViewOp
 
   import opened Options
   import opened Maps
@@ -16,9 +17,9 @@ module GrowModel {
   import opened NativeTypes
 
   /// The root was found to be too big: grow
-  function {:opaque} grow(k: Constants, s: Variables)
-  : (Variables)
-  requires Inv(k, s)
+  function {:opaque} grow(k: Constants, s: BCVariables)
+  : (BCVariables)
+  requires BCInv(k, s)
   requires s.Ready?
   requires BT.G.Root() in s.cache
   requires |s.ephemeralIndirectionTable.graph| <= IndirectionTableModel.MaxSize() - 2
@@ -50,15 +51,15 @@ module GrowModel {
     )
   }
 
-  lemma growCorrect(k: Constants, s: Variables)
-  requires Inv(k, s)
+  lemma growCorrect(k: Constants, s: BCVariables)
+  requires BCInv(k, s)
   requires s.Ready?
   requires BT.G.Root() in s.cache
   requires TotalCacheSize(s) <= MaxCacheSize() - 1
   requires |s.ephemeralIndirectionTable.graph| <= IndirectionTableModel.MaxSize() - 2
   ensures var s' := grow(k, s);
-    && WFVars(s')
-    && M.Next(Ik(k), IVars(s), IVars(s'), UI.NoOp, D.NoDiskOp)
+    && WFBCVars(s')
+    && betree_next(k, IBlockCache(s), IBlockCache(s'))
   {
     reveal_grow();
 
@@ -70,7 +71,7 @@ module GrowModel {
       && s.frozenIndirectionTable.Some?
       && IndirectionTableModel.HasEmptyLoc(s.frozenIndirectionTable.value, BT.G.Root())
     ) {
-      assert noop(k, IVars(s), IVars(s));
+      assert noop(k, IBlockCache(s), IBlockCache(s));
       return;
     }
 
@@ -81,7 +82,7 @@ module GrowModel {
 
     match newref {
       case None => {
-        assert noop(k, IVars(s), IVars(s1));
+        assert noop(k, IBlockCache(s), IBlockCache(s1));
       }
       case Some(newref) => {
         var newroot := Node([], Some([newref]), [B(map[])]);
@@ -101,10 +102,9 @@ module GrowModel {
         var growth := BT.RootGrowth(INode(oldroot), newref);
         assert INode(newroot) == BT.G.Node([], Some([growth.newchildref]), [B(map[])]);
         var step := BT.BetreeGrow(growth);
-        BC.MakeTransaction2(Ik(k), IVars(s), IVars(s1), IVars(s'), BT.BetreeStepOps(step));
-        assert BBC.BetreeMove(Ik(k), IVars(s), IVars(s'), UI.NoOp, M.IDiskOp(D.NoDiskOp), step);
-        assert stepsBetree(k, IVars(s), IVars(s'), UI.NoOp, step);
-        assert stepsBetree(k, IVars(s), IVars(s'), UI.NoOp, step);
+        BC.MakeTransaction2(Ik(k).bc, IBlockCache(s), IBlockCache(s1), IBlockCache(s'), BT.BetreeStepOps(step));
+        assert BBC.BetreeMove(Ik(k).bc, IBlockCache(s), IBlockCache(s'), BlockDisk.NoDiskOp, AdvanceOp(UI.NoOp, true), step);
+        assert stepsBetree(k, IBlockCache(s), IBlockCache(s'), AdvanceOp(UI.NoOp, true), step);
       }
     }
   }
