Impl/SyncModel.i.dfy
@@ -412,7 +412,7 @@ module SyncModel {
     && (froze ==> BBC.Next(Ik(k).bc, IBlockCache(s), IBlockCache(s'), IDiskOp(diskOp(io')).bdop, FreezeOp))
     && (!froze ==>
       || BBC.Next(Ik(k).bc, IBlockCache(s), IBlockCache(s'), IDiskOp(diskOp(io')).bdop, StatesInternalOp)
-      || BBC.Next(Ik(k).bc, IBlockCache(s), IBlockCache(s'), IDiskOp(diskOp(io')).bdop, AdvanceOp(UI.NoOp, false))
+      || BBC.Next(Ik(k).bc, IBlockCache(s), IBlockCache(s'), IDiskOp(diskOp(io')).bdop, AdvanceOp(UI.NoOp, true))
     )
   {
     var (s', io', froze) := maybeFreeze(k, s, io);
@@ -625,7 +625,7 @@ module SyncModel {
   ensures (froze ==> BBC.Next(Ik(k).bc, IBlockCache(s), IBlockCache(s'), IDiskOp(diskOp(io')).bdop, FreezeOp))
   ensures (!froze ==>
     || BBC.Next(Ik(k).bc, IBlockCache(s), IBlockCache(s'), IDiskOp(diskOp(io')).bdop, StatesInternalOp))
-    || BBC.Next(Ik(k).bc, IBlockCache(s), IBlockCache(s'), IDiskOp(diskOp(io')).bdop, AdvanceOp(UI.NoOp, false))
+    || BBC.Next(Ik(k).bc, IBlockCache(s), IBlockCache(s'), IDiskOp(diskOp(io')).bdop, AdvanceOp(UI.NoOp, true))
 
   ensures froze ==> s.frozenIndirectionTable.None?
   {
